%!TEX program = xelatex
\documentclass[lang=en,11pt,a4paper,citestyle =authoryear]{elegantpaper}

% 标题
\title{Homework0 - Paquette}
\author{Boren(Wells) Guan}

% 本文档命令
\usepackage{array,url,stix}
\usepackage{subfigure,listings}
\newcommand{\ccr}[1]{\makecell{{\color{#1}\rule{1cm}{1cm}}}}
\newcommand{\code}[1]{\lstinline{#1}}
\newcommand{\prvd}{$\hfill \qedsymbol$}
\newcommand{\Z}{\mathbb{Z}}
\newcommand{\R}{\mathbb{R}}
\newcommand{\N}{\mathbb{N}}
\newcommand{\C}{\mathbb{C}}
\newcommand{\Q}{\mathbb{Q}}
\newcommand{\M}{\mathcal{M}}
\newcommand{\B}{\mathcal{B}}
\newcommand{\X}{\mathcal{X}}
\newcommand{\Hil}{\mathcal{H}}
\newcommand{\range}{\mathcal{R}}
\newcommand{\nul}{\mathcal{N}}
\newcommand{\F}{\mathcal{F}}

% 文档区
\begin{document}

% 标题
\maketitle

\subsection*{Exercise.1}Show there is a unique solition of the Dyson equation on $\mathbb{M}^+(n)$ given by
\[
M = s(z)I\quad\text{where }s(z):=\dfrac{-z+\sqrt{z-2}\sqrt{z+2}}{2}
\]
with $\sqrt{}$ the princial branch of the square root.
\begin{proof}
    It is easy to see that $M = f(z)I$ for some $f$ and also
    \[
    f(z)(-f(z) - z) = 1
    \]
    and hence $f(z)^2 - zf(z) + 1 = 0$ which means
    \[
    (f(z) - z/2)^2 = (z-2)(z+2)/4
    \]
    for all $z \in \mathbb{H}$.
\end{proof}

\subsection*{Exercise.2} For the Newton flow, suppose that $s(t) = \dfrac{1}{n}tr(\mathcal{M})(t)$. Show that formally
\[
\dfrac{ds(t)}{dt} = \dfrac{e^{-t}\dfrac{1}{n}tr(\xi)}{2s(t)+z}
\]
\begin{proof}
    We know
    \[
    \dfrac{d}{dt} \mathcal{M}(t)(-tr(\mathcal{M}(t))/n - zI_n)  = -\mathcal{M}(t)(-tr(\mathcal{M}(t))/n - zI_n)
    \]
    and we take the trace of the both side we will have
    \[
    \dfrac{d}{dt}(tr(\mathcal{M}(t))(-tr(\mathcal(M)(t)-nz))) = - tr(\mathcal(M)(t))(-tr(\mathcal{M}(t))- nz) 
    \]
    and we will have
    \[
    \dfrac{d}{dt}(s(t)(-s(t)-z)) = -s(t)(-s(t)-z)
    \]
    and hence
    \[
    s'(t)= -\dfrac{s(t)^2-zs(t)}{2s(t)+z}
    \]
\end{proof}

\subsection*{Exercise.3}Conclude that there is an absolute constant $c>0$ so that for any $z\in\mathbb{H}$ if $|2s(z)+z|^2 > c|\dfrac{1}{n}tr(\xi)|$ then the Newton flow is well-posed for all $t\in [0,\infty)$ and
\[
|s(0)- s(\infty)| \leq \dfrac{|\dfrac{1}{n}tr(\xi)|}{\sqrt{|2s(z)+z|^2 - c|\dfrac{1}{n}tr(\xi)|}}
\] 
\begin{proof}
    We have
    \[
    d(2s(t)+z)^2/dt = 2e^{-t}\dfrac{1}{n}tr(\xi) 
    \]
    and hence
    \[
    (2s(t)+z)^2|^{\infty}_0 = -2\dfrac{1}{n}tr(\xi) e^{-t}|^{\infty}_0 = \dfrac{2}{n}tr(\xi)
    \]
    and we have $s(0) = $
\end{proof}

\addappheadtotoc

\end{document}
